Arithmetic/theories/Oracle.v
@@ -12,18 +12,21 @@ Module Type Oracle.
 
     Parameter get_Γᵢ : fsl_pgrm -> Γᵢ. (* static analysis *)
 
-    Parameter 𝓘 : ℨ -> Γᵢ -> 𝐼. (* oracle *)
+    Parameter oracle : ℨ -> Γᵢ -> 𝐼. (* oracle *) (* using 𝓘 messes up vscoq *)
 
     Parameter ϴ :  𝐼 -> 𝔗.
 
-    Definition 𝒯 : ℨ -> Γᵢ -> 𝔗 := fun t τᵢ =>  ϴ (𝓘 t τᵢ).
+    Parameter ϴ_int_or_mpz : forall i, ϴ i = C_Int \/  ϴ i = T_Ext Mpz.
+
+    Definition get_ty : ℨ -> Γᵢ -> 𝔗 := fun t τᵢ =>  ϴ (oracle t τᵢ). (* using 𝒯 messes up vscoq *)
+
 
     Parameter ty_funcall_is_ty_body: 
-        forall S (f : @fenv _fsl_statement S) fname xargs (targs:list ℨ) (iargs:list 𝐼) b, 
+        forall (f : fsl_prog_fenv) fname xargs (targs:list ℨ) (iargs:list 𝐼) b, 
         StringMap.find fname f.(lfuns) = Some (xargs,b) ->
         forall te,
-        List.Forall2 (fun e => eq (𝓘 e te)) targs iargs ->
-                    𝒯 (T_Call fname targs) te = 𝒯 b (StringMap.add_all xargs iargs StringMap.empty).
+        List.Forall2 (fun e => eq (oracle e te)) targs iargs ->
+                    get_ty (T_Call fname targs) te = get_ty b (StringMap.add_all xargs iargs StringMap.empty).
 
 
     (* a term always fits in an mpz and only fits in a machine integer if it is in range *)
@@ -34,7 +37,7 @@ Module Type Oracle.
 
 
     Parameter type_soundness : forall env te f t z, 
-        fsl_term_sem f env t z -> fits z (𝒯 t te).
+        fsl_term_sem f env t z -> fits z (get_ty t te).
 
 
     (* 
@@ -44,17 +47,17 @@ Module Type Oracle.
     Parameter convergence_of_lfuns_ty : 
         forall fname (targs:list ℨ) (iargs:list 𝐼), 
         forall (typing_envs : Ensemble Γᵢ)  (fe:Γᵢ), Ensembles.In Γᵢ typing_envs fe ->
-        (exists ty te, 𝒯 (T_Call fname targs) te = ty) -> 
+        (exists ty te, get_ty (T_Call fname targs) te = ty) -> 
         Finite_sets.Finite _ typing_envs
     .
 
 
     (* fixme: there is also convergence for predicates but the oracle is for terms, not predicates, what to do? *)
     (* Parameter convergence_of_pred_ty : 
-    forall S (f : @fenv _fsl_statement S) pname xargs (targs:list ℨ) (iargs:list 𝐼) b, 
+    forall S (f : fsl_prog_fenv) pname xargs (targs:list ℨ) (iargs:list 𝐼) b, 
     f.(preds) pname = Some (xargs,b) ->
     forall (typing_envs : Ensemble Γᵢ)  (fe:Γᵢ), Ensembles.In Γᵢ typing_envs fe ->
-    (exists ty te, eq (𝒯  (P_Call pname targs) te) ty) -> 
+    (exists ty te, eq (get_ty  (P_Call pname targs) te) ty) -> 
     Finite_sets.Finite _ typing_envs
     . *)
 
