Arithmetic/theories/Languages/MiniC/Syntax.v
@@ -118,7 +118,7 @@ Notation "'if' cond _then 'else' _else " := (If cond _then _else)
     (in custom c_stmt at level 89, cond custom c_exp at level 99, _then custom c_stmt at level 99, _else custom c_stmt at level 99
     , format "'if'  cond '//' '[v '  _then ']' '//' 'else' '//' '[v '  _else ']'") : mini_c_scope.
 Notation "s1 ';' s2" := (Seq s1 s2) (in custom c_stmt at level 90, right associativity, format "s1 ; '//' s2") : mini_c_scope.
-Notation "x = y" := (Assign x y) (in custom c_stmt at level 0, x constr at level 0, y custom c_exp at level 85, no associativity) : mini_c_scope.
+Notation "x := y" := (Assign x y) (in custom c_stmt at level 0, x constr at level 0, y custom c_exp at level 85, no associativity, only printing) : mini_c_scope.
 Notation "'assert' e" := (PAssert e) (in custom c_stmt at level 0, e custom c_exp at level 99) : mini_c_scope.
 Notation "'while' e s" := (While e s) (in custom c_stmt at level 89, e custom c_exp at level 99, s at level 99) : mini_c_scope.
 Notation "'return' e" := (Return e) (in custom c_stmt at level 0, e custom c_exp at level 99) : mini_c_scope.
